tests/lean/run/arrayDecEq.lean
@@ -1,0 +1,27 @@
+def listL (a : Array α) := if a = #[] then 1 else 2
+def listR (a : Array α) := if #[] = a then 1 else 2
+
+/-- info: 1 -/
+#guard_msgs in #eval @listL Nat #[]
+/-- info: 2 -/
+#guard_msgs in #eval listL #[""]
+/-- info: 1 -/
+#guard_msgs in #eval @listL Nat #[]
+/-- info: 2 -/
+#guard_msgs in #eval listL #[()]
+
+section
+variable {α : Type u} [DecidableEq α]
+
+-- test for instance diamonds
+
+/-
+example (x : Array α) :
+    Array.instDecidableEq x #[] = Array.instDecidableEqEmp x := by
+  with_reducible_and_instances rfl
+
+example (x : Array α) :
+    Array.instDecidableEq #[] x = Array.instDecidableEmpEq x := by
+  with_reducible_and_instances rfl
+end
+-/
