tests/lean/run/listDecEq.lean
@@ -1,3 +1,29 @@
+def listL (a : List α) := if a = [] then 1 else 2
+def listR (a : List α) := if [] = a then 1 else 2
+
+/-- info: 1 -/
+#guard_msgs in #eval @listL Nat []
+/-- info: 2 -/
+#guard_msgs in #eval listL [""]
+/-- info: 1 -/
+#guard_msgs in #eval @listL Nat []
+/-- info: 2 -/
+#guard_msgs in #eval listL [()]
+
+section
+variable {α : Type u} [DecidableEq α]
+
+-- test for instance diamonds
+
+example (x : List α) :
+    instDecidableEqList x [] = instDecidableEqNil x := by
+  with_reducible_and_instances rfl
+
+example (x : List α) :
+    instDecidableEqList [] x = instDecidableNilEq x := by
+  with_reducible_and_instances rfl
+end
+
 -- List decidable equality using `withPtrEqDecEq`
 def listDecEqAux {α} [s : DecidableEq α] : ∀ (as bs : List α), Decidable (as = bs)
 | [],    []    => isTrue rfl
