tests/lean/run/optionDecEq.lean
@@ -1,3 +1,16 @@
+def optL (a : Option α) := if a = .none then 1 else 2
+def optR (a : Option α) := if .none = a then 1 else 2
+
+/-- info: 1 -/
+#guard_msgs in #eval @optL Nat .none
+/-- info: 2 -/
+#guard_msgs in #eval optL (some ())
+/-- info: 1 -/
+#guard_msgs in #eval @optR Bool .none
+/-- info: 2 -/
+#guard_msgs in #eval optR (some 1.5)
+
+section
 variable {α : Type u} [DecidableEq α]
 
 -- test for instance diamonds
@@ -9,3 +22,4 @@ example (x : Option α) :
 example (x : Option α) :
     Option.instDecidableEq none x = Option.decidableNoneEq x := by
   with_reducible_and_instances rfl
+end
